lots of progress

cedar-lean/Cedar/Thm/Validation/EntityManifest/Analysis.lean
@@ -1,160 +1,45 @@
-/-
- Copyright Cedar Contributors
 
- Licensed under the Apache License, Version 2.0 (the "License");
- you may not use this file except in compliance with the License.
- You may obtain a copy of the License at
+import Cedar.Spec
 
-      https://www.apache.org/licenses/LICENSE-2.0
-
- Unless required by applicable law or agreed to in writing, software
- distributed under the License is distributed on an "AS IS" BASIS,
- WITHOUT WARRANTIES OR CONDITIONS OF ANY KIND, either express or implied.
- See the License for the specific language governing permissions and
- limitations under the License.
--/
-
-import Cedar.Spec.Expr
-
-import Cedar.Validation.Types
-import Cedar.Data.List
-
-namespace Cedar.Validation.EntityManifest
+namespace Cedar.Thm
 
 open Cedar.Spec
-open Cedar.Validation
-open Cedar.Data
 
-/--
-Stores the access term's constructor and children.
+theorem straight_line_slicing_sound {e : Expr} {s : Entities} {r : Request}
+  {es : StraightLineExprs}
+  {sliced : Entities}
+  : es = (to_straight_line_exprs e) ->
+  sliced =  (simple_slice_entities_straight_line es s) -> evaluate e r s =
+  evaluate e r sliced
+:=
+  sorry
 
-Includes leaf nodes (literals, variables, and strings)
-as well as attribute accesses, tag accesses, and ancestor accesses.
--/
-inductive AccessTerm : Type where
-  -- Literal entity ids
-  | literal (euid : EntityUID)
-  -- A Cedar variable
-  | var (v : Var)
-  -- A literal Cedar string
-  | string (s : String)
-  -- A record or entity attribute
-  | attribute (of : AccessTerm) (attr : Attr)
-  -- An entity tag access
-  | tag (of : AccessTerm) (tag : AccessTerm)
-  -- Whether this entity has a particular ancestor is requested
-  | ancestor (of : AccessTerm) (ancestor : AccessTerm)
-deriving Inhabited, Repr, DecidableEq
+theorem straight_line_slicing_sound_for_straight {se : StraightLineExpr} {s : Entities} {r : Request}
+  {es : StraightLineExprs}
+  {sliced : Entities}
+  : es.contains se ->
+  sliced =  (simple_slice_entities_straight_line es s) -> evaluate es r s =
+  evaluate es r sliced
+:=
+  sorry
 
 
-
-/--
-Like a Cedar Expr, but without if statements.
-Instead, we have droppedCondition, which record the fact that a condition
-was evaluated on the side.
-
-Every Cedar expression is the same as evaluating a StraitLineExpr, with
-if statements replaced with the then or else branch that gets evaluated.
--/
-inductive StraightLineExpr : Type where
-  | lit (p : Prim)
-  | var (v : Var)
-  | droppedCondition (cond : StraightLineExpr) (branchTaken : StraightLineExpr)
-  | and (a : StraightLineExpr) (b : StraightLineExpr)
-  | or (a : StraightLineExpr) (b : StraightLineExpr)
-  | unaryApp (op : UnaryOp) (expr : StraightLineExpr)
-  | binaryApp (op : BinaryOp) (a : StraightLineExpr) (b : StraightLineExpr)
-  | getAttr (expr : StraightLineExpr) (attr : Attr)
-  | hasAttr (expr : StraightLineExpr) (attr : Attr)
-  | set (ls : List StraightLineExpr)
-  | record (map : List (Attr × StraightLineExpr))
-  | call (xfn : ExtFun) (args : List StraightLineExpr)
-
-def StraitLineExprs : Type := Set StraightLineExpr
-
-
-deriving instance Repr, Inhabited for StraightLineExpr
-deriving instance Repr, Inhabited for StraitLineExprs
-
-namespace WrappedAccessTerms
+theorem straight_line_exists_non_erroring {e: Expr} {r: Request}
+  {es : StraightLineExprs } {se : StraightLineExpr} {s: EntityStore}
+  : es = (to_straight_line_exprs e) ->
+    ∃ se,
+    (es.contains se = true) ∧
+      evaluate_straight_line_expr se r s = Some v
+   :=
+  sorry
 
 
 
-mutual
-  def to_straight_line_map_list (exprList: List (Attr × Expr)) : List (List StraightLineExpr) :=
-    match exprList with
-    | [] => []
-    | [x] => [(to_straight_line_exprs x.2).toList]
-    | ele :: rest =>
-      (to_straight_line_exprs ele.2).toList :: (to_straight_line_map_list rest)
-
-  def to_strait_line_list (exprList : List Expr) : List (List StraitLineExpr) :=
-    match exprList with
-    | [] => []
-    | [x] => [(to_straight_line_exprs x).toList]
-    | ele :: rest =>
-      (to_straight_line_exprs ele).toList :: (to_straight_line_map_list rest)
-  /--
-  Converts an expr to a set of strait line exprs,
-  exploring all possibilities when an if statement is encountered.
-  -/
-  def to_straight_line_exprs (expr: Expr) : StraitLineExprs :=
-    match expr with
-    | .ite cond then_expr else_expr =>
-      let cond_exprs := to_straight_line_exprs cond
-      let then_exprs := to_straight_line_exprs then_expr
-      let else_exprs := to_straight_line_exprs else_expr
-
-      let then_with_cond := List.productTR cond_exprs.toList then_exprs.toList
-      let else_with_cond := List.productTR cond_exprs.toList else_exprs.toList
-
-      let then_results := then_with_cond.map (fun pair => .droppedCondition pair.1 pair.2)
-      let else_results := else_with_cond.map (fun pair => .droppedCondition pair.1 pair.2)
-
-      .mk (then_results ++ else_results)
-    | .lit p =>
-      .mk [.lit p]
-    | .var v =>
-      .mk [.var v]
-    | .and a b =>
-      let product := List.productTR (to_straight_line_exprs a).toList (to_straight_line_exprs b).toList
-      .mk (product.map (fun pair => .and pair.1 pair.2))
-    | .or a b =>
-      let product := List.productTR (to_straight_line_exprs a).toList (to_straight_line_exprs b).toList
-      .mk (product.map (fun pair => .or pair.1 pair.2))
-    | .unaryApp op expr =>
-      let exprs := to_straight_line_exprs expr
-      .mk (exprs.toList.map (fun e => .unaryApp op e))
-    | .binaryApp op a b =>
-      let a_exprs := to_straight_line_exprs a
-      let b_exprs := to_straight_line_exprs b
-      let product := List.productTR a_exprs.toList b_exprs.toList
-      .mk (product.map (fun pair => .binaryApp op pair.1 pair.2))
-    | .getAttr expr attr =>
-      let exprs := to_straight_line_exprs expr
-      .mk (exprs.toList.map (fun e => .getAttr e attr))
-    | .hasAttr expr attr =>
-      let exprs := to_straight_line_exprs expr
-      .mk (exprs.toList.map (fun e => .hasAttr e attr))
-    | .set ls =>
-      let exprs_lists := ls.map (fun sete => (to_straight_line_exprs sete).toList)
-      let all_combinations := List.cartesianProduct exprs_lists
-      .mk (all_combinations.map (fun combo => .set combo))
-    | .record map =>
-      let expr_lists := to_straight_line_map_list map
-      let attrs := map.map (fun pair => pair.1)
-      let all_combinations := List.cartesianProduct expr_lists
-      .mk (all_combinations.map (fun combo =>
-        .record (List.zipWith (fun attr expr => (attr, expr)) attrs combo)))
-    | .call xfn args =>
-      let args_exprs := args.map (fun e => (to_straight_line_exprs e).toList)
-      let all_combinations := List.cartesianProduct args_exprs
-      .mk (all_combinations.map (fun combo => .call xfn combo))
-end
-
-
-
-
-end WrappedAccessTerms
-
-end Cedar.Validation.EntityManifest
+theorem straight_line_same_semantics {e: Expr} {r: Request}
+  {es : StraightLineExprs } {se : StraightLineExpr} {s: EntityStore}
+  : es = (to_straight_line_exprs e) ->
+    (es.contains se = true) ->
+      (evaluate_straight_line_expr se r s = Some v) -> -- only when not erroring
+        (evaluate e r s = v)
+   :=
+  sorry
